theories/examples/mutable_typed_shared_data/load.v
@@ -2,39 +2,39 @@ From iris.proofmode Require Import proofmode.
 From cap_machine Require Import fundamental logrel macros macros_helpers proofmode rules register_tactics.
 From cap_machine.examples.mutable_typed_shared_data Require Import dynamic_checks invariants.
 
-Section load_int.
+Section load_cap.
   Context {Σ:gFunctors} {memg:memG Σ} {regg:regG Σ} {sealsg: sealStoreG Σ}
           {nainv: logrel_na_invs Σ} `{MP: MachineParameters}.
 
-  (* Instructions to load in `r_t2` the integer store in the seal `r_t2`, sealed by the `WSealRange` in `r_t1`. *)
+  (* Instructions to load in `r_t2` the capability store in the seal `r_t2`, sealed by the `WSealRange` in `r_t1`. *)
   (* > Beware: The registers are NOT cleared. *)
-  Definition load_global_macro_int_instrs :=
+  Definition load_global_macro_cap_instrs :=
     encodeInstrsW [
       UnSeal r_t2 r_t1 r_t2;
       Load r_t2 r_t2
     ].
 
-  (* Instructions to load in `r_t1` the integer store in the seal `r_t1`, sealed by the hidden `WSealRange` placed at `off_seal`. *)
+  (* Instructions to load in `r_t1` the capability store in the seal `r_t1`, sealed by the hidden `WSealRange` placed at `off_seal`. *)
   (* This will return a new sealed value in `r_t1` and override the registers r_t2`. *)
-  Definition load_global_macro_int_closure_instrs (off_seal : Z) :=
+  Definition load_global_macro_cap_closure_instrs (off_seal : Z) :=
     encodeInstrsW [
       Mov r_t2 r_t1;
       Mov r_t1 PC;
       Lea r_t1 (off_seal - 1)%Z;
       Load r_t1 r_t1
-    ] ++ load_global_macro_int_instrs ++ encodeInstrsW [
+    ] ++ load_global_macro_cap_instrs ++ encodeInstrsW [
       Mov r_t1 r_t2;
       Mov r_t2 0;
       Jmp r_t0
     ].
 
-  Lemma load_global_macro_int_spec
+  Lemma load_global_macro_cap_spec
     p_pc b_pc e_pc a_pc       (* PC *)
     a_cap                     (* Address *)
     p_seal b_seal e_seal τ Φ  (* Seal capability *)
     φ:
 
-    let instrs := load_global_macro_int_instrs in
+    let instrs := load_global_macro_cap_instrs in
     let scap := SCap RW a_cap (a_cap ^+ 1)%a a_cap in
 
     ExecPCPerm p_pc →
@@ -51,16 +51,16 @@ Section load_int.
       ∗ r_t2 ↦ᵣ WSealed τ scap
 
       ∗ ▷ (valid_sealed (WSealed τ scap) τ Φ)
-      ∗ seal_pred_int τ
+      ∗ seal_pred_cap τ
       ∗ na_own logrel_nais ⊤
 
       ∗ ▷ (PC ↦ᵣ WCap p_pc b_pc e_pc (a_pc ^+ (length instrs))%a
              ∗ codefrag a_pc instrs
 
              ∗ r_t1 ↦ᵣ WSealRange p_seal b_seal e_seal τ
-             ∗ (∃ w, r_t2 ↦ᵣ w ∗ ⌜is_z w⌝)
+             ∗ (∃ w, r_t2 ↦ᵣ w ∗ ⌜is_cap w⌝ ∗ interp w)
 
-             ∗ sealed_int (WSealable scap)
+             ∗ sealed_cap (WSealable scap)
              ∗ na_own logrel_nais ⊤
 
              -∗ WP Seq (Instr Executable) {{ λ v, φ v }})
@@ -76,36 +76,37 @@ Section load_int.
 
     iInstr "Hprog".
 
-    iAssert (sealed_int (WSealable scap)) as "#Hseal_int".
+    iAssert (sealed_cap (WSealable scap)) as "#Hseal_cap".
     { iDestruct "Hseal_valid" as (x) "(%Heq & _ & _ & HΦ)".
       inversion Heq; subst.
       iSpecialize ("Heqv" $! (WSealable scap)).
       iRewrite "Heqv".
       iFrame "HΦ". }
 
-    iMod (na_inv_acc with "Hseal_int Hna") as "(>Hseal & Hna & Hclose)"; [ solve_ndisj .. |].
-    iDestruct "Hseal" as (w) "(%Heq & (% & Haddr & %))".
+    iMod (na_inv_acc with "Hseal_cap Hna") as "(Hseal & Hna & Hclose)"; [ solve_ndisj .. |].
+    iDestruct "Hseal" as (w) "(>%Heq & Hseal)".
+    iDestruct "Hseal" as (?) "(>Haddr & >% & #Hseal_interp)".
     case: Heq => _ _ <-.
 
     iGo "Hprog".
 
-    iMod ("Hclose" with "[Haddr $Hna]") as "Hna".
+    iMod ("Hclose" with "[Haddr Hseal_interp $Hna]") as "Hna".
     { iExists _; iSplitR; [ done |].
-      by iExists _; iFrame. }
+      by iExists _; iFrame "# ∗". }
 
     iApply "Hφ".
     iFrame.
     iSplitL "Hr_t2"; eauto.
   Qed.
 
-  Lemma load_global_macro_int_closure_spec (off_seal : Z)
+  Lemma load_global_macro_cap_closure_spec (off_seal : Z)
     p_pc b_pc e_pc a_pc  (* PC *)
-    a_seal a_cap         (* Address *)
+    a_seal a_cap         (* Addresses *)
     p_seal τ Φ           (* Seal capability *)
     adv w2               (* Values in registers *)
     φ:
 
-    let instrs := load_global_macro_int_closure_instrs off_seal in
+    let instrs := load_global_macro_cap_closure_instrs off_seal in
     let scap := SCap RW a_cap (a_cap ^+ 1)%a a_cap in
 
     ExecPCPerm p_pc →
@@ -128,17 +129,17 @@ Section load_int.
       ∗ r_t2 ↦ᵣ w2
 
       ∗ ▷ (valid_sealed (WSealed τ scap) τ Φ)
-      ∗ seal_pred_int τ
+      ∗ seal_pred_cap τ
       ∗ na_own logrel_nais ⊤
 
       ∗ ▷ (PC ↦ᵣ updatePcPerm adv
              ∗ region_mapsto a_pc (a_pc ^+ length instrs)%a instrs
 
              ∗ r_t0 ↦ᵣ adv
-             ∗ (∃ w, r_t1 ↦ᵣ w ∗ ⌜is_z w⌝)
+             ∗ (∃ w, r_t1 ↦ᵣ w ∗ ⌜is_cap w⌝ ∗ interp w)
              ∗ r_t2 ↦ᵣ WInt 0
 
-             ∗ sealed_int (WSealable scap)
+             ∗ sealed_cap (WSealable scap)
              ∗ na_own logrel_nais ⊤
 
              -∗ WP Seq (Instr Executable) {{ λ v, φ v }})
@@ -161,10 +162,10 @@ Section load_int.
 
     focus_block 1%nat "Hprog" as addr_block1 Haddr_block1 "Hblock" "Hcont".
 
-    iApply load_global_macro_int_spec; last iFrame "Hseal_valid ∗"; eauto.
+    iApply load_global_macro_cap_spec; last iFrame "Hseal_valid ∗"; eauto.
 
-    iIntros "!> (HPC & Hblock & Hr_t1 & Hr_t2 & Hseal_int & Hna)".
-    iDestruct "Hr_t2" as (v) "(Hr_t2 & %)".
+    iIntros "!> (HPC & Hblock & Hr_t1 & Hr_t2 & Hseal_cap & Hna)".
+    iDestruct "Hr_t2" as (v) "(Hr_t2 & ?)".
 
     unfocus_block "Hblock" "Hcont" as "Hprog".
 
@@ -180,14 +181,14 @@ Section load_int.
     by iExists _; iFrame.
   Qed.
 
-  Lemma load_global_macro_int_closure_spec_full (off_seal : Z)
+  Lemma load_global_macro_cap_closure_spec_full (off_seal : Z)
     p_pc b_pc e_pc a_pc  (* PC *)
-    a_seal a_cap         (* Address *)
+    a_seal a_cap         (* Addresses *)
     p_seal τ             (* Seal capability *)
     adv w2               (* Values in registers *)
     rmap:
 
-    let instrs := load_global_macro_int_closure_instrs off_seal in
+    let instrs := load_global_macro_cap_closure_instrs off_seal in
     let scap := SCap RW a_cap (a_cap ^+ 1)%a a_cap in
 
     ExecPCPerm p_pc →
@@ -211,10 +212,10 @@ Section load_int.
       ∗ r_t1 ↦ᵣ WSealed τ scap ∗ interp (WSealed τ scap)
       ∗ r_t2 ↦ᵣ w2
 
-      ∗ seal_pred_int τ
+      ∗ seal_pred_cap τ
       ∗ na_own logrel_nais ⊤
 
-      ∗ ([∗ map] r_i↦w_i ∈ rmap, r_i ↦ᵣ w_i ∗ ⌜is_z w_i⌝)
+      ∗ ([∗ map] r_i↦w_i ∈ rmap, r_i ↦ᵣ w_i ∗ interp w_i)
 
       -∗ WP Seq (Instr Executable)
             {{ v, ⌜v = HaltedV⌝ → ∃ r: Reg, full_map r ∧ registers_mapsto r ∗ na_own logrel_nais ⊤ }})%I.
@@ -228,24 +229,19 @@ Section load_int.
     { iDestruct (interp_valid_sealed with "Hseal_interp") as (Φ) "Hseal_valid".
       by iExists Φ. }
 
-    iApply load_global_macro_int_closure_spec; last iFrame; eauto.
+    iApply load_global_macro_cap_closure_spec; last iFrame; eauto.
 
-    iIntros "!> (HPC & Hprog & Hr_t0 & Hr_t1 & Hr_t2 & Hseal_int & Hna)".
-    iDestruct "Hr_t1" as (v) "Hr_t1".
+    iIntros "!> (HPC & Hprog & Hr_t0 & Hr_t1 & Hr_t2 & Hseal_cap & Hna)".
+    iDestruct "Hr_t1" as (v) "(Hr_t1 & _ & Hinterp)".
 
-    iApply "Cont"; eauto; iFrame; revgoals.
-    { iAssert (⌜is_z (WInt 0)⌝)%I as "H"; [ done |].
-      iCombine "Hr_t2 H" as "Hr_t2".
-      iInsertList "Hrmap" [r_t2; r_t1].
+    iApply "Cont"; [| iFrame "HPC Hna" ]; revgoals.
+    { iAssert (interp (WInt 0)) as "Hinterp_int".
+      { by rewrite !fixpoint_interp1_eq. }
 
-      iDestruct (big_sepM_mono _ (λ r w, r ↦ᵣ w ∗ interp w)%I with "[Hrmap]") as "Hrmap"; [| iFrame |].
-      { iIntros (r w Hrmap) "(Hr & %Hr_int)".
-        iFrame.
-        destruct w; [| by simpl in Hr_int.. ].
-        by rewrite fixpoint_interp1_eq. }
-
+      iCombine "Hr_t2 Hinterp_int" as "Hr_t2".
+      iCombine "Hr_t1 Hinterp" as "Hr_t1".
       iCombine "Hr_t0 Hadv_interp" as "Hr_t0".
-      iInsertList "Hrmap" [r_t0].
+      iInsertList "Hrmap" [r_t0; r_t1; r_t2].
 
       iFrame. }
 
@@ -255,4 +251,4 @@ Section load_int.
     set_solver +.
   Qed.
 
-End load_int.
+End load_cap.
